src/CertifiedExtraction/Benchmarks/ProcessScheduler.v
@@ -1,0 +1,164 @@
+Require Import Fiat.ADT.Core.
+Require Import Bedrock.Platform.Facade.DFModule.
+Require Import Fiat.ADTNotation.
+Require Import Bedrock.Platform.Facade.CompileUnit2.
+Require Import Fiat.Common.i3list.
+Require Import Fiat.Common.ilist3.
+
+Require Import
+        CertifiedExtraction.Core
+        CertifiedExtraction.FacadeUtils
+        CertifiedExtraction.StringMapUtils
+        CertifiedExtraction.Extraction.Internal
+        CertifiedExtraction.Extraction.Extraction
+        CertifiedExtraction.Extraction.QueryStructures
+        CertifiedExtraction.ADT2CompileUnit.
+
+Definition State := W.
+Definition SLEEPING : State := Word.natToWord 32 0.
+Definition RUNNING : State  := Word.natToWord 32 1.
+
+Instance : Query_eq (Word.word n) :=
+  { A_eq_dec := @Word.weq n }.
+Opaque Word.weq.
+
+Definition SchedulerSchema :=
+  Query Structure Schema [
+          relation "Processes" has schema
+          <"pid" :: W, "state" :: State, "cpu" :: W>
+          where (UniqueAttribute ``"pid")
+  ] enforcing [].
+
+Definition SchedulerSpec : ADT _ :=
+  QueryADTRep SchedulerSchema {
+    Def Constructor0 "Init" : rep := empty,
+
+    Def Method3 "Spawn" (r : rep) (new_pid cpu state : W) : rep * bool :=
+      Insert (<"pid" :: new_pid, "state" :: state, "cpu" :: cpu> : RawTuple) into r!"Processes",
+
+    Def Method1 "Enumerate" (r : rep) (state : State) : rep * list W :=
+      procs <- For (p in r!"Processes")
+               Where (p!"state" = state)
+               Return (p!"pid");
+      ret (r, procs),
+
+    Def Method1 "GetCPUTime" (r : rep) (id : W) : rep * list W :=
+        proc <- For (p in r!"Processes")
+                Where (p!"pid" = id)
+                Return (p!"cpu");
+      ret (r, proc)
+              }%methDefParsing.
+
+Definition SharpenedScheduler :
+  MostlySharpened SchedulerSpec.
+Proof.
+  start sharpening ADT.
+  simpl; pose_string_hyps; pose_heading_hyps.
+  start_honing_QueryStructure'.
+  hone method "Spawn".
+  { setoid_rewrite UniqueAttribute_symmetry.
+    setoid_rewrite (@refine_uniqueness_check_into_query' SchedulerSchema Fin.F1 _ _ _ _).
+    setoid_rewrite refine_For_rev.
+    setoid_rewrite refine_Count.
+    simplify with monad laws; simpl in *; subst.
+    setoid_rewrite refine_pick_eq'.
+    setoid_rewrite refine_bind_unit.
+    setoid_rewrite refine_If_Then_Else_Duplicate.
+    finish honing. }
+  (* Now we implement the various set operations using BagADTs. *)
+  - make_simple_indexes
+      {|
+      prim_fst := [ ("EqualityIndex", Fin.FS (@Fin.F1 1) );
+                    ( "EqualityIndex", Fin.F1) ];
+      prim_snd := () |}
+               ltac:(LastCombineCase6 BuildEarlyEqualityIndex)
+                      ltac:(LastCombineCase5 BuildLastEqualityIndex).
+    + plan EqIndexUse createEarlyEqualityTerm createLastEqualityTerm
+           EqIndexUse_dep createEarlyEqualityTerm_dep createLastEqualityTerm_dep.
+    + plan EqIndexUse createEarlyEqualityTerm createLastEqualityTerm
+           EqIndexUse_dep createEarlyEqualityTerm_dep createLastEqualityTerm_dep.
+    + setoid_rewrite refine_For_rev; simplify with monad laws.
+      plan EqIndexUse createEarlyEqualityTerm createLastEqualityTerm
+           EqIndexUse_dep createEarlyEqualityTerm_dep createLastEqualityTerm_dep.
+    + setoid_rewrite refine_For_rev; simplify with monad laws.
+      plan EqIndexUse createEarlyEqualityTerm createLastEqualityTerm
+           EqIndexUse_dep createEarlyEqualityTerm_dep createLastEqualityTerm_dep.
+    + hone method "Spawn".
+      { subst; simplify with monad laws.
+        unfold GetAttributeRaw at 1.
+        simpl; unfold ilist2_hd at 1; simpl.
+        unfold H1; apply refine_under_bind.
+        intros; set_evars.
+        setoid_rewrite refine_pick_eq'; simplify with monad laws.
+        rewrite app_nil_r, map_map; simpl.
+        unfold ilist2_hd; simpl; rewrite map_id.
+        repeat setoid_rewrite refine_If_Then_Else_Bind.
+        repeat setoid_rewrite refineEquiv_bind_unit; simpl.
+        setoid_rewrite refineEquiv_bind_bind.
+        setoid_rewrite refineEquiv_bind_unit.
+        rewrite (CallBagFind_fst H0); simpl.
+        finish honing.
+      }
+      hone method "Enumerate".
+      { subst; simplify with monad laws.
+        unfold H1; apply refine_under_bind.
+        intros; set_evars; simpl in *.
+        rewrite (CallBagFind_fst H0).
+        setoid_rewrite refine_pick_eq'; simplify with monad laws.
+        simpl; rewrite app_nil_r, map_map, <- map_rev.
+        unfold ilist2_hd; simpl.
+        finish honing.
+      }
+      hone method "GetCPUTime".
+      { subst; simplify with monad laws.
+        unfold H1; apply refine_under_bind.
+        intros; set_evars; rewrite (CallBagFind_fst H0); simpl in *.
+        setoid_rewrite refine_pick_eq'; simplify with monad laws.
+        simpl; rewrite app_nil_r, map_map, <- map_rev.
+        unfold ilist2_hd; simpl.
+        finish honing.
+      }
+      simpl.
+      eapply reflexivityT.
+  - unfold CallBagFind, CallBagInsert.
+    pose_headings_all;
+      match goal with
+      | |- appcontext[ @BuildADT (IndexedQueryStructure ?Schema ?Indexes) ] =>
+        FullySharpenQueryStructure Schema Indexes
+      end.
+Defined.
+
+Time Definition PartialSchedulerImpl : ADT _ :=
+  Eval simpl in (fst (projT1 SharpenedScheduler)).
+Print PartialSchedulerImpl.
+
+Time Definition SchedulerImplSpecs :=
+  Eval simpl in (Sharpened_DelegateSpecs (snd (projT1 SharpenedScheduler))).
+Print SchedulerImplSpecs.
+
+Definition CUnit
+  : { env : _ &
+    BuildCompileUnit2TSpec
+      env
+      (AbsR (fst (projT2 SharpenedScheduler)))
+      (fun r => BagSanityConditions (prim_fst r))
+      (DecomposeIndexedQueryStructure' QsADTs.ADTValue _ _)
+      (DecomposeIndexedQueryStructurePre' QsADTs.ADTValue _ _ _)
+      (DecomposeIndexedQueryStructurePost' QsADTs.ADTValue _ _ (Scheduler_RepWrapperT _))
+      (QueryStructureSchema.numQSschemaSchemas SchedulerSchema)
+      "foo"
+      "bar"
+      Scheduler_coDomainWrappers
+      Scheduler_DomainWrappers
+      (Scheduler_RepWrapperT _)
+      (Scheduler_DecomposeRep_well_behaved QsADTs.ADTValue _ _ (Scheduler_RepWrapperT _))
+      (fst (projT2 SharpenedScheduler))} .
+Proof.
+  Time _compile QSEnv_Ax.
+Time Defined.
+
+(* Set Printing All. *)
+
+Redirect "SpawnSmall" Eval compute in (projT1 CUnit).
+Redirect "EnumerateSmall" Eval compute in (projT1 (progOKs (Fin.FS Fin.F1))).
+Redirect "GetCPUTimeSmall" Eval compute in (projT1 (progOKs (Fin.FS (Fin.FS Fin.F1)))).
